theory Test

imports Main

begin

lemma "2 + 2 = 4" by simp

lemma "1 + 1 = 2" by simp

lemma "2 + 2 = 4" by simp

lemma "1 + 1 = 2" by simp
lemma "2 + 2 = 4" by simp

lemma "1 + 1 = 2" by simp
lemma "2 + 2 = 4" by simp

lemma "1 + 1 = 2" by simp
lemma "2 + 2 = 4" by simp

lemma "1 + 1 = 2" by simp
lemma "2 + 2 = 4" by simp

lemma "1 + 1 = 2" by simp
lemma "2 + 2 = 4" by simp

lemma "1 + 1 = 2" by simp
lemma "2 + 2 = 4" by simp

lemma "1 + 1 = 2" by simp
lemma "2 + 2 = 4" by simp

lemma "1 + 1 = 2" by simp
lemma "2 + 2 = 4" by simp

lemma "1 + 1 = 2" by simp
lemma "2 + 2 = 4" by simp

lemma "1 + 1 = 2" by simp
lemma "2 + 2 = 4" by simp

lemma "                                                   True" by simp

lemma "1 + 1 = 2" by simp
lemma "2 + 2 = 4" by simp

lemma "1 + 1 = 2" by simp
lemma "2 + 2 = 4" by simp

lemma "1 + 1 = 2" by simp
lemma "2 + 2 = 4" by simp

lemma "1 + 1 = 2" by simp
lemma "2 + 2 = 4" by simp

lemma "1 + 1 = 2" by simp
lemma "2 + 2 = 4" by simp

lemma "1 + 1 = 2" by simp
lemma "2 + 2 = 4" by simp

lemma "1 + 1 = 2" by simp
lemma "2 + 2 = 4" by simp

lemma "1 + 1 = 2" by simp
lemma "2 + 2 = 4" by simp

lemma "1 + 1 = 2" by simp
lemma "2 + 2 = 4" by simp

lemma "1 + 1 = 2" by simp
lemma "2 + 2 = 4" by simp

lemma "1 + 1 = 2" by simp
lemma "2 + 2 = 4" by simp

lemma "1 + 1 = 2" by simp
lemma "2 + 2 = 4" by simp

lemma "1 + 1 = 2" by simp
lemma "2 + 2 = 4" by simp

lemma "1 + 1 = 2" by simp
lemma "2 + 2 = 4" by simp

lemma "1 + 1 = 2" by simp
lemma "2 + 2 = 4" by simp

lemma "1 + 1 = 2" by simp
lemma "2 + 2 = 4" by simp

lemma "1 + 1 = 2" by simp
lemma "2 + 2 = 4" by simp

lemma "1 + 1 = 2" by simp
lemma "2 + 2 = 4" by simp

lemma "1 + 1 = 2" by simp
lemma "2 + 2 = 4" by simp

lemma "1 + 1 = 2" by simp
lemma "2 + 2 = 4" by simp

lemma "1 + 1 = 2" by simp
lemma "2 + 2 = 4" by simp

lemma "1 + 1 = 2" by simp
lemma "2 + 2 = 4" by simp

lemma "1 + 1 = 2" by simp
lemma "2 + 2 = 4" by simp

lemma "1 + 1 = 2" by simp
lemma "2 + 2 = 4" by simp

lemma "1 + 1 = 2" by simp
lemma "2 + 2 = 4" by simp

lemma "1 + 1 = 2" by simp
lemma "2 + 2 = 4" by simp

lemma "1 + 1 = 2" by simp
lemma "2 + 2 = 4" by simp

lemma "1 + 1 = 2" by simp
lemma "2 + 2 = 4" by simp

lemma "1 + 1 = 2" by simp
lemma "2 + 2 = 4" by simp

lemma "1 + 1 = 2" by simp
lemma "2 + 2 = 4" by simp

lemma "1 + 1 = 2" by simp
lemma "2 + 2 = 4" by simp

lemma "1 + 1 = 2" by simp
lemma "2 + 2 = 4" by simp

lemma "1 + 1 = 2" by simp
lemma "2 + 2 = 4" by simp

lemma "1 + 1 = 2" by simp
lemma "2 + 2 = 4" by simp

lemma "1 + 1 = 2" by simp
lemma "2 + 2 = 4" by simp

lemma "1 + 1 = 2" by simp
lemma "2 + 2 = 4" by simp

lemma "1 + 1 = 2" by simp
lemma "2 + 2 = 4" by simp

lemma "1 + 1 = 2" by simp
lemma "2 + 2 = 4" by simp

lemma "1 + 1 = 2" by simp
lemma "2 + 2 = 4" by simp

lemma "1 + 1 = 2" by simp
lemma "2 + 2 = 4" by simp

lemma "1 + 1 = 2" by simp
lemma "2 + 2 = 4" by simp

lemma "1 + 1 = 2" by simp
lemma "2 + 2 = 4" by simp

lemma "1 + 1 = 2" by simp
lemma "2 + 2 = 4" by simp

lemma "1 + 1 = 2" by simp
lemma "2 + 2 = 4" by simp

lemma "\<exists>x. x = 5" by blast

lemma "x = y \<longrightarrow> y = x" by simp

lemma test: "1 = 1" by simp

lemma "(\<exists>x. x = 5 \<and> x = y) \<Longrightarrow> y = 5" by auto

lemma "1 + 2 = 3" by simp
lemma "2 + 2 = 4" using list.induct list.induct by simp

lemma "1 + 1 = 2" by simp
lemma "2 + 2 = 4" by simp

lemma "1 + 1 = 2" by simp
lemma "2 + 2 = 4" by simp

lemma "1 + 1 = 2" by simp
lemma "2 + 2 = 4" by simp

lemma "1 + 1 = 2" by simp
lemma "2 + 2 = 4" by simp

lemma "1 + 1 = 2" by simp
lemma "2 + 2 = 4" by simp

lemma "1 + 1 = 2" by simp
lemma "2 + 2 = 4" by simp

lemma "1 + 1 = 2" by simp
lemma "2 + 2 = 4" by simp

lemma "1 + 1 = 2" by simp
lemma "2 + 2 = 4" by simp

lemma "1 + 1 = 2" by simp
lemma "2 + 2 = 4" by simp

lemma "1 + 1 = 2" by simp
lemma "2 + 2 = 4" by simp

lemma "1 + 1 = 2" by simp
lemma "2 + 2 = 4" by simp

lemma "1 + 1 = 2" by simp
lemma "2 + 2 = 4" by simp

lemma "1 + 1 = 2" by simp
lemma "2 + 2 = 4" by simp

lemma "1 + 1 = 2" by simp
lemma "2 + 2 = 4" by simp

lemma "1 + 1 = 2" by simp
lemma "2 + 2 = 4" by simp

lemma "1 + 1 = 2" by simp
lemma "2 + 2 = 4" by simp

lemma "1 + 1 = 2" by simp
lemma "2 + 2 = 4" by simp

lemma "1 + 1 = 2" by simp
lemma "2 + 2 = 4" by simp

lemma "1 + 1 = 2" by simp
lemma "2 + 2 = 4" by simp

lemma "1 + 1 = 2" by simp
lemma "2 + 2 = 4" by simp

lemma "1 + 1 = 2" by simp
lemma "2 + 2 = 4" by simp

lemma "1 + 1 = 2" by simp
lemma "2 + 2 = 4" by simp

lemma "1 + 1 = 2" by simp
lemma "2 + 2 = 4" by simp

lemma "1 + 1 = 2" by simp
lemma "2 + 2 = 4" by simp

lemma "1 + 1 = 2" by simp
lemma "2 + 2 = 4" by simp

lemma "1 + 1 = 2" by simp
lemma "2 + 2 = 4" by simp

lemma "1 + 1 = 2" by simp
lemma "2 + 2 = 4" by simp

lemma "1 + 1 = 2" by simp
lemma "2 + 2 = 4" by simp

lemma "1 + 1 = 2" by simp
lemma "2 + 2 = 4" by simp

lemma "1 + 1 = 2" by simp
lemma "2 + 2 = 4" by simp

lemma "1 + 1 = 2" by simp
lemma "2 + 2 = 4" by simp

lemma "1 + 1 = 2" by simp
lemma "2 + 2 = 4" by simp

lemma "1 + 1 = 2" by simp
lemma "2 + 2 = 4" by simp

lemma "1 + 1 = 2" by simp
lemma "2 + 2 = 4" by simp

lemma "1 + 1 = 2" by simp
lemma "2 + 2 = 4" by simp

lemma "1 + 1 = 2" by simp
lemma "2 + 2 = 4" by simp

lemma "1 + 1 = 2" by simp
lemma "2 + 2 = 4" by simp

lemma "1 + 1 = 2" by simp
lemma "2 + 2 = 4" by simp

lemma "1 + 1 = 2" by simp
lemma "2 + 2 = 4" by simp

lemma "1 + 1 = 2" by simp
lemma "2 + 2 = 4" by simp

lemma "1 + 1 = 2" by simp
lemma "2 + 2 = 4" by simp

lemma "1 + 1 = 2" by simp
lemma "2 + 2 = 4" by simp

lemma "1 + 1 = 2" by simp
lemma "2 + 2 = 4" by simp

lemma "1 + 1 = 2" by simp
lemma "2 + 2 = 4" by simp

lemma "1 + 1 = 2" by simp

end
